examples/containers/hs-spec/IntSetProperties.v
@@ -16,6 +16,9 @@ Require Data.IntSet.Internal.
 Require Test.QuickCheck.Property.
 Require IntSetProofs.
 
+Require String.
+Import String.StringSyntax.
+
 Instance Arbitrary_IntSet : Test.QuickCheck.Property.Arbitrary Data.IntSet.Internal.IntSet :=
   { arbitrary := Test.QuickCheck.Property.MkGen IntSetProofs.WF }.
 
