examples/containers/theories/IntSetWordProofs.v
@@ -8,7 +8,7 @@ Local Open Scope Z_scope.
 Require Import BitUtils.
 Require Import CTZ.
 Require Import DyadicIntervals.
-Require Import Tactics.
+Require Import CustomTactics.
 Require Import OrdTactic.
 
 (** ** Utilities about sorted (specialized to [N.lt]) *)
@@ -191,7 +191,7 @@ Lemma rPrefix_shiftr:
   forall e,
   NToInt (rPrefix (N.shiftr (intToN e) tip_width, tip_width)) = prefixOf e.
 Admitted.
-(* 
+(*
 Proof.
   intros.
   unfold rPrefix, prefixOf, suffixBitMask.
@@ -200,9 +200,9 @@ Proof.
   reflexivity.
 Qed.
 *)
-(*  
+(*
 Lemma prefixOf_eq_shiftr:
-  forall i p, 
+  forall i p,
   (prefixOf i =? N.shiftl p tip_width) = ((N.shiftr i tip_width) =? p).
 Proof.
   intros.
@@ -369,7 +369,7 @@ Proof.
   destruct r as [p b]. simpl in *.
   unfold zero. unfoldMethods.
 Admitted.
-(* 
+(*
   apply N_land_pow2_eq.
 Qed. *)
 
@@ -384,14 +384,14 @@ Lemma nomatch_zero:
   (inRange (intToN i) r = false -> P otherwise) ->
   (inRange (intToN i) (halfRange r false) = true  -> inRange (intToN i) (halfRange r true) = false -> P left) ->
   (inRange (intToN i) (halfRange r false) = false -> inRange (intToN i) (halfRange r true) = true -> P right) ->
-  P (if nomatch i (NToInt (rPrefix r)) (NToInt (rMask r)) then otherwise else 
+  P (if nomatch i (NToInt (rPrefix r)) (NToInt (rMask r)) then otherwise else
      if zero i (NToInt (rMask r)) then left else right).
 Proof.
   intros.
   rewrite nomatch_spec by auto.
   rewrite if_negb.
   destruct (inRange (intToN i) r) eqn:?.
-  * rewrite zero_spec by auto. 
+  * rewrite zero_spec by auto.
     rewrite if_negb.
     destruct (N.testbit (intToN i) (rBits r - 1)) eqn:Hbit.
     + apply H2.
@@ -409,7 +409,7 @@ Lemma nomatch_zero_smaller:
   (rangeDisjoint r1 r = true -> P otherwise) ->
   (isSubrange r1 (halfRange r false) = true  -> isSubrange r1 (halfRange r true) = false -> P left) ->
   (isSubrange r1 (halfRange r false) = false -> isSubrange r1 (halfRange r true) = true -> P right) ->
-  P (if nomatch (NToInt (rPrefix r1)) (NToInt (rPrefix r)) (NToInt (rMask r)) then otherwise else 
+  P (if nomatch (NToInt (rPrefix r1)) (NToInt (rPrefix r)) (NToInt (rMask r)) then otherwise else
      if zero (NToInt (rPrefix r1)) (NToInt (rMask r)) then left else right).
 Proof.
   intros ????????.
@@ -451,7 +451,7 @@ Proof.
   unfold branchMask.
   unfold msDiffBit.
   rewrite N.add_sub.
-Admitted. (* 
+Admitted. (*
   reflexivity.
 Qed. *)
 
@@ -489,7 +489,7 @@ Proof.
   intros.
   destruct r1 as [p1 b1], r2 as [p2 b2]. simpl in *.
 Admitted.
-(*  
+(*
   change ((2 ^ (b2 - 1)) <? (2 ^ (b1 - 1)) = (b2 <? b1)).
   apply eq_true_iff_eq.
   rewrite !N.ltb_lt.
@@ -533,7 +533,7 @@ Proof.
   intros.
   unfold bitmapInRange.
   destruct (inRange i r); try reflexivity.
-Admitted. (* 
+Admitted. (*
   rewrite N.lor_spec; reflexivity.
 Qed. *)
 
@@ -549,13 +549,13 @@ Admitted.
 (*   rewrite N.lxor_spec; reflexivity.
 Qed.
  *)
- 
+
  Lemma bitmapInRange_lnot: (* Misses some precondition *)
   forall r bm i,
     bitmapInRange r (NToWord (N.lnot bm WIDTH)) i =
     negb (bitmapInRange r (NToWord bm) i).
 Admitted.
- 
+
 Lemma bitmapInRange_land:
   forall r bm1 bm2 i,
     bitmapInRange r (NToWord (N.land bm1 bm2)) i =
@@ -564,7 +564,7 @@ Proof.
   intros.
   unfold bitmapInRange.
   destruct (inRange i r); try reflexivity.
-Admitted. (* 
+Admitted. (*
   rewrite N.land_spec; reflexivity.
 Qed. *)
 
@@ -577,7 +577,7 @@ Proof.
   unfold bitmapInRange.
   destruct (inRange i r); try reflexivity.
 Admitted.
-(* 
+(*
   rewrite N.ldiff_spec; reflexivity.
 Qed. *)
 
@@ -596,7 +596,7 @@ Proof.
   rewrite -> N.eqb_sym.
   Int_Word_N.
 Admitted.
-(*  
+(*
   rewrite <- N_eq_shiftr_land_ones.
   apply N.eqb_sym.
 Qed.
@@ -739,7 +739,7 @@ Proof.
   unfold suffixBitMask in H0.
   rewrite H0.
   rewrite N.lor_0_r.
-Admitted. (* 
+Admitted. (*
   reflexivity.
 Qed. *)
 
@@ -790,14 +790,14 @@ Proof.
   * destruct H.
     destruct (N.lt_decidable 0%N (N.log2 bm)).
     - apply N.log2_lt_pow2; try assumption.
-    - assert (N.log2 bm = 0%N) by 
+    - assert (N.log2 bm = 0%N) by
         (destruct (N.log2 bm); auto; contradict H1; reflexivity).
       rewrite H2. reflexivity.
   * apply N.bit_log2.
     unfold isBitMask in *.
     destruct bm; simpl in *; intuition; compute in H1; congruence.
 Qed.
- 
+
 Lemma isBitMask_lor:
   forall bm1 bm2, isBitMask bm1 -> isBitMask bm2 -> isBitMask (N.lor bm1 bm2).
 Proof.
@@ -806,7 +806,7 @@ Proof.
   * destruct (isBitMask_testbit bm1 H) as [j[??]].
     assert (N.testbit (N.lor bm1 bm2) j = true) by
      (rewrite N.lor_spec, H2; auto).
-    enough (0 <> N.lor bm1 bm2)%N by 
+    enough (0 <> N.lor bm1 bm2)%N by
      (destruct (N.lor bm1 bm2); auto; try congruence; apply pos_pos).
     contradict H3; rewrite <- H3.
     rewrite N.bits_0. congruence.
@@ -1068,7 +1068,7 @@ Lemma revNat_ldiff:
 Proof.
   intros.
 Admitted.
-(*  
+(*
   apply N.bits_inj_iff; intro i.
   destruct (N.ltb_spec i WIDTH).
   * rewrite !revNat_spec, !N.ldiff_spec, !revNat_spec; isBitMask.
@@ -1093,7 +1093,7 @@ Lemma revNat_pow:
 Proof.
   intros.
 Admitted.
-(* 
+(*
   apply N.bits_inj_iff; intro j.
   destruct (N.ltb_spec j WIDTH).
   * rewrite !revNat_spec by assumption.
@@ -1150,7 +1150,7 @@ Proof.
   unfold lowestBitMask.
   unfold isBitMask0 in *.
 Admitted.
-(*   
+(*
   apply N.pow_lt_mono_r; try Nomega.
   isBitMask.
 Qed. *)
@@ -1197,7 +1197,7 @@ Proof.
   unfold isBitMask in *. Nomega.
 Qed.
  *)
- 
+
 Lemma split_highestBitMask:
   forall bm,
   isBitMask bm ->
@@ -1389,7 +1389,7 @@ Lemma bits_ind:
   P bm.
 Proof.
   intros bm P Hbm HP0 HPstep.
-  
+
   revert Hbm.
   apply well_founded_ind with (R := N.lt) (a := bm); try apply N.lt_wf_0.
   clear bm. intros bm IH Hbm0.
@@ -1415,7 +1415,7 @@ Lemma bits_ind_up:
   P bm.
 Proof.
   intros bm P Hbm HP0 HPstep.
-  
+
   revert Hbm.
   apply well_founded_ind with (R := N.lt) (a := bm); try apply N.lt_wf_0.
   clear bm. intros bm IH Hbm0.
@@ -1497,7 +1497,7 @@ Inductive Desc : IntSet -> range -> (N -> bool) -> Prop :=
     isSubrange r1 (halfRange r false) = true ->
     isSubrange r2 (halfRange r true) = true ->
     p = NToInt (rPrefix r) ->
-    msk = NToInt (rMask r) -> 
+    msk = NToInt (rMask r) ->
     (forall i, f i = f1 i || f2 i) ->
     Desc (Bin p msk s1 s2) r f.
 
@@ -1640,7 +1640,7 @@ Qed.
 
 
 Lemma isBitMask_bitmapInRange:
-  forall r bm, rBits r = Nlog2 WIDTH -> isBitMask (wordToN bm) ->
+  forall r bm, rBits r = N.log2 WIDTH -> isBitMask (wordToN bm) ->
     exists i, bitmapInRange r bm i = true.
 Proof.
   intros.
@@ -1694,7 +1694,7 @@ Admitted.
 (** This auxillary tactic destructs one boolean atom in the argument *)
 
 Ltac split_bool_go expr :=
-  lazymatch expr with 
+  lazymatch expr with
     | true       => fail
     | false      => fail
     | Some _     => fail
@@ -1711,7 +1711,7 @@ Ltac split_bool_go expr :=
 (** This auxillary tactic destructs one boolean or option atom in the goal *)
 
 Ltac split_bool :=
-  match goal with 
+  match goal with
     | [ |- ?lhs = ?rhs] => split_bool_go lhs || split_bool_go rhs
   end.
 
@@ -1731,15 +1731,15 @@ Ltac solve_f_eq :=
     + (rewrite bitmapInRange_lnot; Int_Word_N)
     + (rewrite bitmapInRange_land; Int_Word_N)
     + (rewrite bitmapInRange_lor; Int_Word_N)
-    + match goal with 
+    + match goal with
       | [ H : forall i : N, ?f i = _ |- context [?f i] ] => rewrite H
       end);
   repeat split_bool;
   try reflexivity.
 
 Ltac point_to_inRange :=
-  lazymatch goal with 
-    | [ HD : Desc ?s ?r ?f, Hf : ?f ?i = true |- _ ] 
+  lazymatch goal with
+    | [ HD : Desc ?s ?r ?f, Hf : ?f ?i = true |- _ ]
       => apply (Desc_inside HD) in Hf
     | [ H : bitmapInRange ?r ?bm ?i = true |- _ ]
       => apply bitmapInRange_inside in H
@@ -1747,7 +1747,7 @@ Ltac point_to_inRange :=
 
 Ltac pose_new prf :=
   let prop := type of prf in
-  match goal with 
+  match goal with
     | [ H : prop |- _] => fail 1
     | _ => pose proof prf
   end.
@@ -1835,7 +1835,7 @@ Proof.
   intros.
   apply isSubrange_antisym.
   + eapply both_halfs with (i1 := i1) (i2 := i2); eassumption.
-  + eapply both_halfs with (i1 := i3) (i2 := i4); eassumption.  
+  + eapply both_halfs with (i1 := i3) (i2 := i4); eassumption.
 Qed.
 
 Lemma larger_f_imp:
@@ -2020,11 +2020,11 @@ Proof.
         -- rewrite (Desc_outside HD1_1) in H4 by inRange_false.
            rewrite orb_false_l in H4.
            rewrite <- H4; clear H4.
-           
+
            rewrite (Desc_outside HD3_1) in H10 by inRange_false.
            rewrite orb_false_l in H10.
            rewrite <- H10; clear H10.
-           
+
            assumption.
         -- rewrite (Desc_outside HD1_2) by inRange_false.
            rewrite (Desc_outside HD3_2) by inRange_false.
@@ -2047,12 +2047,12 @@ Proof.
   destruct H, H0.
   * reflexivity.
   * exfalso.
-    destruct (Desc_some_f HD) as [i Hi]. 
+    destruct (Desc_some_f HD) as [i Hi].
     rewrite <- H1 in Hi.
     rewrite H in Hi.
     congruence.
   * exfalso.
-    destruct (Desc_some_f HD) as [i Hi]. 
+    destruct (Desc_some_f HD) as [i Hi].
     rewrite -> H1 in Hi.
     rewrite H in Hi.
     congruence.
@@ -2217,7 +2217,7 @@ Next Obligation.
        + simpl. omega.
        + eapply DescTip with (p := NToInt (rPrefix r)) (r := r) (bm := bm); try eassumption; try congruence.
        + eassumption.
-       + apply pointwise_iff. intros i Hi. 
+       + apply pointwise_iff. intros i Hi.
          assert (inRange i r = true). {
            rewrite H1 in Hi.
            apply bitmapInRange_inside in Hi.
@@ -2231,7 +2231,7 @@ Next Obligation.
        + simpl. omega.
        + eapply DescTip with (p := NToInt (rPrefix r)) (r := r) (bm := bm); try eassumption; try congruence.
        + eassumption.
-       + apply pointwise_iff. intros i Hi. 
+       + apply pointwise_iff. intros i Hi.
          assert (inRange i r = true). {
            rewrite H1 in Hi.
            apply bitmapInRange_inside in Hi.
@@ -2284,7 +2284,7 @@ Next Obligation.
          + simpl. omega.
          + eapply DescBin with (s1 := s1) (s2 := s0) (r := r); try eassumption; reflexivity.
          + eassumption.
-         + apply pointwise_iff. intros i Hi. 
+         + apply pointwise_iff. intros i Hi.
            assert (inRange i r = true). {
              rewrite H4 in Hi.
              rewrite orb_true_iff in Hi; destruct Hi as [Hi | Hi];
@@ -2299,7 +2299,7 @@ Next Obligation.
          + simpl. omega.
          + eapply DescBin with (s1 := s1) (s2 := s0) (r := r); try eassumption; reflexivity.
          + eassumption.
-         + apply pointwise_iff. intros i Hi. 
+         + apply pointwise_iff. intros i Hi.
            assert (inRange i r = true). {
              rewrite H4 in Hi.
              rewrite orb_true_iff in Hi; destruct Hi as [Hi | Hi];
@@ -2338,7 +2338,7 @@ Next Obligation.
            rewrite orb_false_r in H4.
            assumption.
         ++ specialize (H4 i). specialize (H10 i).
-           rewrite H9 in H4. 
+           rewrite H9 in H4.
            apply (Desc_inside HD1_2) in H9.
            rewrite orb_true_r in H4.
            apply H8 in H4. rewrite H10 in H4.
@@ -2453,7 +2453,7 @@ Proof.
   * erewrite member_Desc; eauto.
 Qed.
 
-Lemma Desc_has_member: 
+Lemma Desc_has_member:
   forall {s r f}, Desc s r f -> exists i, member i s = true.
 Proof.
   intros ??? HD.
@@ -2588,7 +2588,7 @@ Qed.
 Lemma insertBM_Desc:
   forall p' bm r1 f1,
   forall s2 r2 f2,
-  forall r f, 
+  forall r f,
   Desc (Tip p' bm) r1 f1 ->
   Desc s2 r2 f2 ->
   r = commonRange r1 r2 ->
@@ -2638,7 +2638,7 @@ Qed.
 Lemma insert_Desc:
   forall e r1,
   forall s2 r2 f2,
-  forall r f, 
+  forall r f,
   Desc s2 r2 f2 ->
   r1 = (N.shiftr (intToN e) tip_width, tip_width) ->
   r = commonRange r1 r2 ->
@@ -2731,7 +2731,7 @@ Lemma bin_Desc0:
     isSubrange r1 (halfRange r false) = true ->
     isSubrange r2 (halfRange r true) = true ->
     p = NToInt (rPrefix r) ->
-    msk = NToInt (rMask r) -> 
+    msk = NToInt (rMask r) ->
     (forall i, f i = f1 i || f2 i) ->
     Desc0 (bin p msk s1 s2) r f.
 Proof.
@@ -2868,7 +2868,7 @@ Qed.
 (** The following is copied from the body of [union] *)
 
 Definition union_body s1 s2 := match s1, s2 with
-  | (Bin p1 m1 l1 r1 as t1) , (Bin p2 m2 l2 r2 as t2) => 
+  | (Bin p1 m1 l1 r1 as t1) , (Bin p2 m2 l2 r2 as t2) =>
      let union2 :=
        if nomatch p1 p2 m2 : bool
        then link p1 t1 p2 t2
@@ -2913,7 +2913,7 @@ Program Fixpoint union_Desc
   Desc s1 r1 f1 ->
   Desc s2 r2 f2 ->
   (forall i, f i = f1 i || f2 i) ->
-  Desc (union s1 s2) (commonRange r1 r2) f 
+  Desc (union s1 s2) (commonRange r1 r2) f
   := fun HD1 HD2 Hf => _.
 Next Obligation.
   rewrite union_eq.
@@ -3040,7 +3040,7 @@ Proof. now union_Sem_reasoning; rewrite orb_comm. Qed.
 
 (** *** Verification of [unions] *)
 
-Require Import Proofs.Data.Foldable. 
+Require Import Proofs.Data.Foldable.
 
 Lemma Forall_rev:
   forall A P (l : list A), Forall P (rev l) <-> Forall P l.
@@ -3164,7 +3164,7 @@ Program Fixpoint intersection_Desc
   Desc s1 r1 f1 ->
   Desc s2 r2 f2 ->
   (forall i, f i = f1 i && f2 i) ->
-  Desc0 (intersection s1 s2) r1 f 
+  Desc0 (intersection s1 s2) r1 f
   := fun HD1 HD2 Hf => _.
 Next Obligation.
   rewrite intersection_eq.
@@ -3224,7 +3224,7 @@ Next Obligation.
       subst.
 
       (* Now we are essentially in the same situation as above. *)
-      (* Unfortunately, the two implementations of [intersectionBM] are slightly 
+      (* Unfortunately, the two implementations of [intersectionBM] are slightly
          different in irrelevant details that make ist just hard enough to abstract
          over them in a lemma of its own. So let’s just copy’n’paste. *)
       clear intersection_Desc.
@@ -3257,7 +3257,7 @@ Next Obligation.
            ** apply IHHD1_2.
               solve_f_eq_disjoint.
            ** isSubrange_true; eapply Desc_rNonneg; eassumption.
- 
+
     + subst.
       set (sl := Bin (NToInt (rPrefix r1)) (NToInt (rMask r1)) s0 s3) in *.
       set (sr := Bin (NToInt (rPrefix r2)) (NToInt (rMask r2)) s4 s5) in *.
@@ -3377,7 +3377,7 @@ Definition difference_body s1 s2 := match s1, s2 with
   | (Bin _ _ _ _ as t) , Nil => t
   | (Tip kx bm as t1) , t2 =>
      (fix differenceTip arg_12__
-        := match arg_12__ as arg_12__' return (arg_12__' = arg_12__ -> IntSet) with 
+        := match arg_12__ as arg_12__' return (arg_12__' = arg_12__ -> IntSet) with
              | Bin p2 m2 l2 r2 => fun _ =>
                                   if nomatch kx p2 m2 : bool
                                   then t1
@@ -3417,7 +3417,7 @@ Program Fixpoint difference_Desc
   Desc s1 r1 f1 ->
   Desc s2 r2 f2 ->
   (forall i, f i = f1 i && negb (f2 i)) ->
-  Desc0 (difference s1 s2) r1 f 
+  Desc0 (difference s1 s2) r1 f
   := fun HD1 HD2 Hf => _.
 Next Obligation.
   rewrite difference_eq.
@@ -3725,7 +3725,7 @@ Next Obligation.
       subst.
 
       (* Now we are essentially in the same situation as above. *)
-      (* Unfortunately, the two implementations of [intersectionBM] are slightly 
+      (* Unfortunately, the two implementations of [intersectionBM] are slightly
          different in irrelevant details that make ist just hard enough to abstract
          over them in a lemma of its own. So let’s just copy’n’paste. *)
 
@@ -3897,7 +3897,7 @@ Proof.
         rewrite <- prefixOf_eqb_spec in Heqb by assumption.
         rewrite N.eqb_eq in Heqb.
         rewrite N.ltb_ge in Heqb0. subst.
-        apply prefixOf_mono in Heqb0. 
+        apply prefixOf_mono in Heqb0.
         lia.
       + solve_f_eq.
         apply bitmapInRange_inside in Heqb.
@@ -3905,7 +3905,7 @@ Proof.
         rewrite N.eqb_eq in Heqb.
         rewrite N.ltb_lt in Heqb0. subst.
         assert (x <= i) by lia.
-        apply prefixOf_mono in H. 
+        apply prefixOf_mono in H.
         lia.
     - (* s is Tip, x is part of it *)
       assert ((bitmapOf x - 1)%N = (N.ones (suffixOf x)%N)) as Htmp.
@@ -3989,7 +3989,7 @@ Proof.
               rewrite (Desc_outside HD2) by inRange_false.
               reflexivity.
            ++ rewrite andb_false_r. reflexivity.
-        ** intros i. 
+        ** intros i.
            destruct (N.ltb_spec x i).
            ++ rewrite andb_true_r. reflexivity.
            ++ destruct (inRange i r) eqn:Hir; only 1: (apply inRange_bounded in Hir; lia).
@@ -4191,7 +4191,7 @@ Proof.
         rewrite <- prefixOf_eqb_spec in Heqb by assumption.
         rewrite N.eqb_eq in Heqb.
         rewrite N.ltb_ge in Heqb0. subst.
-        apply prefixOf_mono in Heqb0. 
+        apply prefixOf_mono in Heqb0.
         lia.
       + solve_f_eq.
         apply bitmapInRange_inside in Heqb.
@@ -4199,7 +4199,7 @@ Proof.
         rewrite N.eqb_eq in Heqb.
         rewrite N.ltb_lt in Heqb0. subst.
         assert (x <= i) by lia.
-        apply prefixOf_mono in H. 
+        apply prefixOf_mono in H.
         lia.
     - (* s is Tip, x is part of it *)
       assert ((bitmapOf x - 1)%N = (N.ones (suffixOf x)%N)) as Htmp.
@@ -4301,7 +4301,7 @@ Proof.
               rewrite (Desc_outside HD2) by inRange_false.
               reflexivity.
            ++ rewrite andb_false_r. reflexivity.
-        ** intros i. 
+        ** intros i.
            destruct (N.ltb_spec x i).
            ++ rewrite andb_true_r. reflexivity.
            ++ destruct (inRange i r) eqn:Hir; only 1: (apply inRange_bounded in Hir; lia).
@@ -4483,7 +4483,7 @@ Proof.
   f_equal.
   admit.
 Admitted.
-(*  
+(*
   rewrite revNat_revNat.
   reflexivity.
 Qed.
@@ -4503,7 +4503,7 @@ Lemma foldrBits_bm:
   forall {a} p (f : Int -> a -> a) bm x,
   isBitMask (wordToN bm) ->
   foldrBits p f x bm =
-    foldrBits p f (f (ZToInt (intToZ p + Z.of_N (N.log2 (wordToN bm)))%Z) x) 
+    foldrBits p f (f (ZToInt (intToZ p + Z.of_N (N.log2 (wordToN bm)))%Z) x)
         (NToWord (N.clearbit (wordToN bm) (N.log2 (wordToN bm)))).
 Proof.
   intros.
@@ -4747,7 +4747,7 @@ Lemma to_List_Bits_sorted:
 Proof.
   intros.
 Admitted.
-(*  
+(*
   apply bits_ind with (bm := bm).
   * assumption.
   * rewrite foldrBits_0.
@@ -4890,7 +4890,7 @@ Lemma foldlBits_eq:
   forall {a} p (f : a -> Int -> a) x bm,
   foldlBits p f x bm = @foldlBits_go a p f x bm (fun x y => foldlBits p f (proj1_sig y) x).
 Admitted.
-(* This should work once the termiation proof of foldlBits does not use an axiom. *) 
+(* This should work once the termiation proof of foldlBits does not use an axiom. *)
 (*
 Proof.
   intros.
@@ -4911,7 +4911,7 @@ Lemma foldlBits_bm:
   forall {a} p (f : a -> Int -> a) bm x,
   isBitMask (wordToN bm) ->
   foldlBits p f x bm =
-    foldlBits p f 
+    foldlBits p f
        (f x (ZToInt (intToZ p + Z.of_N (N_ctz (wordToN bm)))))
        (NToWord (N.clearbit (wordToN bm) (N_ctz (wordToN bm)))).
 Proof.
@@ -4966,7 +4966,7 @@ Admitted.
   - clear bm H. intros bm Hbm IH _ Hpos x.
     destruct (N.eqb_spec (N.clearbit bm (N_ctz bm)) (0%N)).
     * clear IH.
-    
+
       rewrite foldlBits_bm by isBitMask.
       rewrite e.
       rewrite foldlBits_0.
@@ -5085,10 +5085,10 @@ Qed.
 *)
 
 Lemma fold_right_toList_go:
-  forall {a} f (x : a) s r f' xs, Desc s r f' -> 
+  forall {a} f (x : a) s r f' xs, Desc s r f' ->
   fold_right f x (foldr_go cons xs s) = foldr_go f (fold_right f x xs) s.
 Proof.
-  intros. 
+  intros.
   revert xs; induction H; intros.
   * apply fold_right_foldrBits_go; isBitMask.
   * simpl.
@@ -5098,7 +5098,7 @@ Proof.
 Qed.
 
 Lemma fold_right_toList:
-  forall {a} f (x : a) s xs, WF s-> 
+  forall {a} f (x : a) s xs, WF s->
   fold_right f x (foldr cons xs s) = foldr f (fold_right f x xs) s.
 Proof.
   intros.
@@ -5109,7 +5109,7 @@ Proof.
     + apply fold_right_foldrBits_go; isBitMask.
     + simpl.
       unfoldMethods. Int_Word_N.
-      fold (foldr_go (@cons Key)). 
+      fold (foldr_go (@cons Key)).
       fold (foldr_go f).
       destruct (Z.ltb_spec (intToZ msk) 0).
       - do 2 erewrite fold_right_toList_go by eassumption. reflexivity.
@@ -5156,7 +5156,7 @@ Lemma popCount_N_length_toList_go:
 Proof.
   intros.
   revert l.
-Admitted.  
+Admitted.
 (*
   apply bits_ind with (bm := bm).
   - isBitMask.
@@ -5251,7 +5251,7 @@ Proof.
   intros.
   unfold size.
   rewrite sizeGo_spec by assumption.
-  simpl. Int_Word_N.  
+  simpl. Int_Word_N.
   reflexivity.
 Qed.
 
@@ -5391,7 +5391,7 @@ Qed.
 
 Lemma filter_Desc:
   forall p s r f f',
-  Desc s r f -> 
+  Desc s r f ->
   (forall i, f' i = f i && p (NToInt i)) ->
   Desc0 (filter p s) r f'.
 Proof.
@@ -5443,7 +5443,7 @@ Admitted.
 
 Lemma filter_Sem:
   forall p s f f',
-  Sem s f -> 
+  Sem s f ->
   (forall i, f' i = f i && p (NToInt i)) ->
   Sem (filter p s) f'.
 Proof.
@@ -5566,7 +5566,7 @@ Admitted.
       rewrite <- not_true_iff_false in H1.
       contradict H1.
       rewrite Forall_forall in H2.
-      rewrite isSubsetOf_Sem by eassumption. 
+      rewrite isSubsetOf_Sem by eassumption.
       intros i Hi.
       apply H2.
       rewrite <- toList_In by eassumption.
@@ -5602,7 +5602,7 @@ Proof.
   * do 2 rewrite Sem_notSubset_witness by eassumption.
     intuition.
     + destruct H2 as [i?]. exists i. intuition congruence.
-    + destruct H2 as [i?]. exists i. intuition congruence.    
+    + destruct H2 as [i?]. exists i. intuition congruence.
     + destruct H1 as [i?].
       destruct (f1 i) eqn:?, (f2 i) eqn:?; try congruence.
       - left. exists i. intuition congruence.
@@ -5764,7 +5764,7 @@ Proof.
   eapply Sem_change_f; only 1: eassumption.
   intro i.
   apply eq_iff_eq_true.
-  admit.
+Admitted.
 (*
   rewrite Hf.
   rewrite existsb_exists, in_map_iff.
@@ -6021,7 +6021,7 @@ Instance Ord_WFIntSet : Ord WFIntSet := fun _ k => k
 Ltac unfold_applied t :=
   let rec hd t' := match t' with
                    | ?f _ => hd f
-                   | ?x   => x 
+                   | ?x   => x
                    end in
   let f := hd t      in
   let x := fresh "x" in
@@ -6082,27 +6082,27 @@ Local Ltac to_Ord_list :=
 Instance OrdLaws_WFIntSet : OrdLaws WFIntSet.
 Proof.
   constructor; unfold_WFIntSet_Ord; try now to_Ord_list; order (list N).
-  
+
   - intros [s1 WF1] [s2 WF2]; simpl.
     rewrite !compare_not_Gt_le => LE1 LE2.
     apply equal_spec, toAscList_exact; trivial.
     apply (reflect_iff _ _ (Eq_eq _ _)); generalize dependent LE1; generalize dependent LE2;
       to_Ord_list; order (list N).
-  
+
   - intros [s1 WF1] [s2 WF2]; simpl.
     destruct (Ord_total (toAscList s1) (toAscList s2)); to_Ord_list; order (list N).
-  
+
   - intros [s1 WF1] [s2 WF2]; simpl.
     unfold "==", Eq___IntSet, Data.IntSet.Internal.Eq___IntSet_op_zeze__; simpl.
     rewrite equal_spec, toAscList_exact, Ord_compare_Eq; trivial.
     symmetry; apply (ssrbool.rwP (Eq_eq _ _)).
-  
+
   - intros [s1 WF1] [s2 WF2]; simpl.
     apply eq_iff_eq_true;
       rewrite !compare_not_Gt_le; fold_is_true;
       rewrite <-(ssrbool.rwP (Eq_eq _ _)), Ord_compare_Lt;
       order (list N).
-  
+
   - intros [s1 WF1] [s2 WF2]; simpl.
     apply eq_iff_eq_true;
       rewrite !compare_not_Gt_le; fold_is_true;
@@ -6179,13 +6179,13 @@ Admitted.
 Instance MonoidLaws_WFIntSet : MonoidLaws WFIntSet.
 Proof.
   constructor.
-  - intros [s WFs]; WFIntSet_Eq_eq. 
+  - intros [s WFs]; WFIntSet_Eq_eq.
     now destruct s.
-  - intros [s WFs]; WFIntSet_Eq_eq. 
+  - intros [s WFs]; WFIntSet_Eq_eq.
     now destruct s.
-  - intros [s1 WF1] [s2 WF2]; WFIntSet_Eq_eq. 
+  - intros [s1 WF1] [s2 WF2]; WFIntSet_Eq_eq.
     reflexivity.
-  - intros ss; WFIntSet_Eq_eq. 
+  - intros ss; WFIntSet_Eq_eq.
     unfold mconcat, Monoid__IntSet, Data.IntSet.InternalWord.Monoid__IntSet_mconcat; simpl.
     unfold unions; rewrite hs_coq_foldl_list', hs_coq_foldr_base, hs_coq_map.
     induction ss as [|s ss IH]; simpl.
@@ -6231,9 +6231,9 @@ Module IntSetFSet <: WSfun(Int_as_OT) <: WS <: Sfun(Int_as_OT) <: S.
   Definition elt := Int.
 
   (* Well-formedness *)
-  
+
   Definition t := WFIntSet.
-  
+
   Notation "x <-- f ;; P" :=
     (match f with
      | exist x _ => P
@@ -6243,7 +6243,7 @@ Module IntSetFSet <: WSfun(Int_as_OT) <: WS <: Sfun(Int_as_OT) <: S.
 
   Definition In_set x (s : IntSet) :=
     member x s = true.
-  
+
   Definition In x (s' : t) :=
     s <-- s' ;;
     In_set x s.
@@ -6252,36 +6252,36 @@ Module IntSetFSet <: WSfun(Int_as_OT) <: WS <: Sfun(Int_as_OT) <: S.
   Definition Equal s s' := forall a : elt, In a s <-> In a s'.
 
   Definition eq : t -> t -> Prop := Equal.
-  
+
   Definition Subset s s' := forall a : elt, In a s -> In a s'.
   Definition Empty s := forall a : elt, ~ In a s.
 
   Definition empty : t.
     eexists. eexists. apply SemNil. intro. reflexivity.
   Defined.
-  
-  Definition is_empty : t -> bool := fun s' => 
+
+  Definition is_empty : t -> bool := fun s' =>
     s <-- s' ;; null s.
 
   (* IntSet comparison predicate *)
-  
+
   Definition lt (s s' : t) : Prop := (s < s') = true.
-  
+
   (* More information later, after we've proved theorems *)
 
   (* Minimal and maximal elements *)
-  
+
   (* Definition min_elt : t -> option elt := fmap fst ∘ minView ∘ unpack. *)
-  
+
   (* Definition max_elt : t -> option elt := fmap fst ∘ maxView ∘ unpack. *)
-  
+
   (* The bit-twiddling to prove `minView` and `maxView` correct is quite
      difficult.  In the meantime: *)
-  
+
   Definition min_elt : t -> option elt := @hd_error _ ∘ toAscList ∘ unpack.
-  
+
   Definition max_elt : t -> option elt := @hd_error _ ∘ toDescList ∘ unpack.
-  
+
   (* Theorems *)
 
   Lemma empty_1 : Empty empty.
@@ -6350,7 +6350,7 @@ Module IntSetFSet <: WSfun(Int_as_OT) <: WS <: Sfun(Int_as_OT) <: S.
     fun ws ws' => s <-- ws ;;
                s' <-- ws' ;;
                s == s'.
-  
+
   Definition subset : t -> t -> bool :=
     fun ws ws' => s <-- ws ;;
                s' <-- ws' ;;
@@ -6387,7 +6387,7 @@ Module IntSetFSet <: WSfun(Int_as_OT) <: WS <: Sfun(Int_as_OT) <: S.
   Proof. destruct s. unfold eq. unfold Equal. intro. reflexivity. Qed.
 
   Lemma eq_sym : forall s s' : t, eq s s' -> eq s' s.
-  Proof. destruct s; destruct s'; 
+  Proof. destruct s; destruct s';
     unfold eq, Equal in *. intros. rewrite H. intuition. Qed.
 
   Lemma eq_trans :
@@ -6433,7 +6433,7 @@ Module IntSetFSet <: WSfun(Int_as_OT) <: WS <: Sfun(Int_as_OT) <: S.
   Lemma In_1 :
     forall (s : t) (x y : elt), Int_as_OT.eq x y -> In x s -> In y s.
   Proof. intros. destruct H. assumption. Qed.
-  
+
   Definition mem : elt -> t -> bool := fun e s' =>
    s <-- s' ;; member e s.
 
@@ -6443,7 +6443,7 @@ Module IntSetFSet <: WSfun(Int_as_OT) <: WS <: Sfun(Int_as_OT) <: S.
 
   Lemma mem_2 : forall (s : t) (x : elt), mem x s = true -> In x s.
   Proof. unfold In; intros; destruct s as [s]; auto. Qed.
-  
+
   Lemma equal_1 : forall s s' : t, Equal s s' -> equal s s' = true.
   Proof.
     intros.
@@ -6695,7 +6695,7 @@ Module IntSetFSet <: WSfun(Int_as_OT) <: WS <: Sfun(Int_as_OT) <: S.
     rewrite andb_true_iff in H.
     intuition.
   Qed.
-  
+
   Lemma inter_3 :
     forall (s s' : t) (x : elt), In x s -> In x s' -> In x (inter s s').
   Proof.
@@ -6893,19 +6893,19 @@ Module IntSetFSet <: WSfun(Int_as_OT) <: WS <: Sfun(Int_as_OT) <: S.
     rewrite <- toList_In in H by eassumption.
     assumption.
   Qed.
-  
+
   Lemma elements_3 (s : t) : Sorted E.lt (elements s).
   Proof.
     unfold E.lt; destruct s as [s WFs]; simpl.
     apply StronglySorted_Sorted.
     now apply to_List_sorted.
   Qed.
-  
+
   Lemma elements_3w (s : t) : NoDupA Int_as_OT.eq (elements s).
   Proof. apply OrdFacts.Sort_NoDup, elements_3. Qed.
-  
+
   (* Ordering theorems *)
-  
+
   Definition compare (s s' : t) : Compare lt eq s s'.
   Admitted.
   (* Needs OrdLaws *)
@@ -6918,14 +6918,14 @@ Module IntSetFSet <: WSfun(Int_as_OT) <: WS <: Sfun(Int_as_OT) <: S.
     - apply GT; abstract order t.
   Defined.
   *)
-  
+
   Theorem lt_trans (s1 s2 s3 : t) :
     lt s1 s2 -> lt s2 s3 -> lt s1 s3.
   Admitted.
   (*
-  Proof. unfold lt; order t. Qed. 
+  Proof. unfold lt; order t. Qed.
   *)
-  
+
   Theorem lt_not_eq (s1 s2 : t) :
     lt s1 s2 -> ~ eq s1 s2.
   Admitted.
@@ -6939,7 +6939,7 @@ Module IntSetFSet <: WSfun(Int_as_OT) <: WS <: Sfun(Int_as_OT) <: S.
     order WFIntSet.
   Qed.
   *)
-  
+
   Lemma min_elt_1 (s : t) (x : elt) : min_elt s = Some x -> In x s.
   Proof.
     destruct s as [s [fs SEM_s]]; unfold min_elt, "∘"; simpl; unfold In_set.
@@ -6948,7 +6948,7 @@ Module IntSetFSet <: WSfun(Int_as_OT) <: WS <: Sfun(Int_as_OT) <: S.
     eapply toList_In; [eassumption|].
     now unfold toList; rewrite ASC; left.
   Qed.
-  
+
   Lemma min_elt_2 (s : t) (x y : elt) : min_elt s = Some x -> In y s -> ~ E.lt y x.
   Proof.
     destruct s as [s WFs]; destruct (WFs) as [fs SEM_s]; unfold min_elt, "∘", E.lt; simpl; unfold In_set.
@@ -6963,7 +6963,7 @@ Module IntSetFSet <: WSfun(Int_as_OT) <: WS <: Sfun(Int_as_OT) <: S.
     - specialize (min_x _ IN_y).
       specialize (Z.lt_trans _ _ _ LT min_x); apply Z.lt_irrefl.
   Qed.
-  
+
   Lemma min_elt_3 (s : t) : min_elt s = None -> Empty s.
   Proof.
     destruct s as [s [fs SEM_s]]; unfold min_elt, "∘", Empty; simpl; unfold In_set.
@@ -6982,7 +6982,7 @@ Module IntSetFSet <: WSfun(Int_as_OT) <: WS <: Sfun(Int_as_OT) <: S.
     eapply toList_In, in_rev; [eassumption|].
     now fold Key; rewrite DESC; left.
   Qed.
-  
+
   Lemma max_elt_2 (s : t) (x y : elt) : max_elt s = Some x -> In y s -> ~ E.lt x y.
   Proof.
     destruct s as [s WFs]; destruct (WFs) as [fs SEM_s]; unfold max_elt, "∘", E.lt; simpl; unfold In_set.
@@ -6998,7 +6998,7 @@ Module IntSetFSet <: WSfun(Int_as_OT) <: WS <: Sfun(Int_as_OT) <: S.
     - specialize (max_x _ IN_y).
       specialize (Z.lt_trans _ _ _ LT max_x); apply Z.lt_irrefl.
   Qed.
-  
+
   Lemma max_elt_3 (s : t) : max_elt s = None -> Empty s.
   Proof.
     destruct s as [s WFs]; destruct (WFs) as [fs SEM_s]; unfold max_elt, "∘", Empty; simpl; unfold In_set.
@@ -7008,7 +7008,7 @@ Module IntSetFSet <: WSfun(Int_as_OT) <: WS <: Sfun(Int_as_OT) <: S.
     erewrite member_Sem, toList_In, in_rev by eassumption.
     now fold Key; rewrite DESC.
   Qed.
-  
+
   (**
   These (non-ordering) portions of the [FSetInterface]s have no counterpart in the [IntSet] interface.
   We implement them generically.
@@ -7121,7 +7121,7 @@ Module IntSetFSet <: WSfun(Int_as_OT) <: WS <: Sfun(Int_as_OT) <: S.
   Qed.
 
   Lemma choose_3 (s1 s2 : t) (x1 x2 : elt) :
-    choose s1 = Some x1 -> 
+    choose s1 = Some x1 ->
     choose s2 = Some x2 ->
     Equal s1 s2         ->
     E.eq  x1 x2.
