examples/containers/theories/MapProofs/Common.v
@@ -1,0 +1,8 @@
+Require Export GHC.Base.
+Export GHC.Base.Notations.
+Require Export Proofs.GHC.Base.
+Require Export Data.Map.Internal.
+Export GHC.Num.Notations.
+Require Export OrdTactic.
+Require Export Psatz.
+Require Export CustomTactics.
