examples/containers/theories/MapProofs/TypeclassProofs.v
@@ -1,11 +1,4 @@
-Require Import GHC.Base.
-Import GHC.Base.Notations.
-Require Import Proofs.GHC.Base.
-Require Import Data.Map.Internal.
-Import GHC.Num.Notations.
-Require Import OrdTactic.
-Require Import Psatz.
-Require Import Tactics.
+Require Import MapProofs.Common.
 Set Bullet Behavior "Strict Subproofs".
 Require Import MapProofs.Bounds.
 Require Import MapProofs.MapFunctionProofs.
@@ -51,7 +44,7 @@ Instance OrdLaws_Pair {a} {b} `{OrdLaws a} `{OrdLaws b} : OrdLaws (a * b).
 Proof.
   constructor.
   - intros. destruct a1. destruct b0. unfold "<=", "==" in *. unfold Ord_pair___, Eq_pair___ in *.
-    unfold ord_default, op_zeze____  in *. simpl in *. rewrite andb_true_iff.  rewrite negb_true_iff in *. 
+    unfold ord_default, op_zeze____  in *. simpl in *. rewrite andb_true_iff.  rewrite negb_true_iff in *.
     destruct (compare a2 a1) eqn : ?. destruct (compare b0 b1) eqn : ?.
     rewrite compare_Eq in Heqc. rewrite compare_Eq in Heqc0. split.
     apply Eq_Symmetric. apply Heqc. apply Eq_Symmetric. apply Heqc0.
@@ -64,7 +57,7 @@ Proof.
     unfold compare_pair in *. unfold ord_default in *. simpl in *. rewrite negb_true_iff in *.
     repeat (try (destruct (compare a2 a1) eqn : ?); try (destruct (compare b2 b1) eqn : ?);
     try (destruct (compare a3 a1) eqn : ?); try (destruct (compare b0 b1) eqn : ?);
-    try (destruct (compare a2 a3) eqn : ?); try (destruct (compare b2 b0) eqn : ?); 
+    try (destruct (compare a2 a3) eqn : ?); try (destruct (compare b2 b0) eqn : ?);
     try (order b); try (order a0)).
   - intros. destruct a1. destruct b0. unfold "<=" in *. unfold Ord_pair___ in *. unfold compare_pair in *.
     unfold ord_default. unfold ord_default in *. simpl. rewrite negb_true_iff. rewrite negb_true_iff.
@@ -74,7 +67,7 @@ Proof.
     right. destruct (compare a1 a2) eqn : ?. order a0. order a0. reflexivity.
     left. reflexivity.
   - intros. unfold compare.   unfold "<=" in *. unfold Ord_pair___ in *. unfold compare_pair in *.
-    unfold ord_default. simpl. rewrite negb_false_iff. destruct a1. destruct b0. 
+    unfold ord_default. simpl. rewrite negb_false_iff. destruct a1. destruct b0.
     split; intros. destruct (compare a1 a2). rewrite H1. reflexivity. reflexivity. inversion H1.
     destruct (compare a1 a2). destruct (compare b1 b0). inversion H1. reflexivity. inversion H1.
     reflexivity. inversion H1.
@@ -84,7 +77,7 @@ Proof.
     split; assumption. inversion H1. inversion H1. rewrite andb_true_iff in H1. destruct H1.
     inversion H. inversion H0. apply Ord_compare_Eq in H1. apply Ord_compare_Eq0 in H2. rewrite H1. assumption.
   - intros. unfold compare. unfold Ord_pair___ , "<=". unfold compare_pair. unfold ord_default. simpl.
-    destruct a1. destruct b0. split; intros. rewrite negb_false_iff.  
+    destruct a1. destruct b0. split; intros. rewrite negb_false_iff.
     destruct (compare a1 a2) eqn : ?. assert (compare a2 a1 = Eq) by (order a0). rewrite H2.
     assert (compare b0 b1 = Lt) by (order b). rewrite H3. reflexivity. inversion H1. inversion H1.
     assert (compare a2 a1 = Lt) by (order a0). rewrite H2. reflexivity.
@@ -209,9 +202,9 @@ Proof.
     match goal with |- context[?b = true] => fold (is_true b) end.
     rewrite <-(ssrbool.rwP (Eq_eq _ _)).
     order (list (e * a)).
-  - intros. unfold Internal.Ord__Map_op_zl__, "/=". unfold Internal.Ord__Map_compare, 
+  - intros. unfold Internal.Ord__Map_op_zl__, "/=". unfold Internal.Ord__Map_compare,
     Eq_comparison___. unfold op_zsze____ . rewrite negb_involutive. destruct (compare _ _) eqn : ?;
-    unfold eq_comparison; unfold proj1_sig in *; destruct a0; destruct b. 
+    unfold eq_comparison; unfold proj1_sig in *; destruct a0; destruct b.
     assert (compare (toAscList x0) (toAscList x) = Eq) by (order (list (e * a))). rewrite H0.
     reflexivity.  assert (compare (toAscList x0) (toAscList x) = Gt) by (order (list (e * a))).
     rewrite H0. reflexivity. assert (compare (toAscList x0) (toAscList x) = Lt) by (order (list (e * a))).
@@ -307,16 +300,16 @@ Proof.
     apply H2. erewrite <- map_preserves_size. erewrite <- map_preserves_size. apply H3.
     apply H0. apply H. erewrite <- map_preserves_size. erewrite <- map_preserves_size.
     apply H4. apply H0. apply H.
-Qed. 
+Qed.
 
 Lemma map_preserves_WF : forall {b} {c} (m : Map e b) (f : b -> c),
   WF m -> WF (map f m).
-Proof. 
+Proof.
   intros. unfold WF in *. apply map_bounded. apply H.
-Qed. 
+Qed.
 
 
-Definition Functor__Map_fmap 
+Definition Functor__Map_fmap
    : forall {a} {b}, (a -> b) -> (Map e) a -> (Map e) b :=
   fun {a} {b} => fun f m => map f m.
 
@@ -327,12 +320,12 @@ Local Definition Functor__map_op_zlzd__
 Lemma const_WF: forall {b} {a: Type} (x : a) (m: Map e b),
   WF m -> WF (map (const x) m).
 Proof.
-  intros. apply map_preserves_WF. apply H. 
+  intros. apply map_preserves_WF. apply H.
 Qed.
 
 
 Global Program Instance Functor_Map : Functor (WFMap e) :=
-  fun _ k => 
+  fun _ k =>
   k {| GHC.Base.fmap__ := fun {a} => @fmap (Map e) _ _ ;
         GHC.Base.op_zlzd____ := fun {a} {b} x => @fmap (Map e) _ b a (@const a b _) |}.
 Next Obligation.
@@ -344,19 +337,19 @@ Qed.
 
 Global Instance FunctorLaws_MapWF: FunctorLaws (WFMap e).
   constructor.
-  - intros. destruct x. unfold fmap. unfold fmap__.  unfold Functor_Map. 
+  - intros. destruct x. unfold fmap. unfold fmap__.  unfold Functor_Map.
     apply ProofIrrelevance.ProofIrrelevanceTheory.subset_eq_compat. unfold proj1_sig.
     unfold fmap. unfold fmap__. unfold Functor__Map. unfold Internal.Functor__Map_fmap.
-    induction w. 
+    induction w.
     + simpl. reflexivity.
     + simpl. rewrite IHw1. rewrite IHw2. reflexivity.
   - intros. destruct x. unfold fmap in *. unfold fmap__ in *.
     unfold Functor_Map in *. apply ProofIrrelevance.ProofIrrelevanceTheory.subset_eq_compat.
-    unfold proj1_sig in *. unfold fmap. unfold Functor__Map. unfold fmap__. 
+    unfold proj1_sig in *. unfold fmap. unfold Functor__Map. unfold fmap__.
     unfold Internal.Functor__Map_fmap. simpl. induction w.
     + simpl. reflexivity.
     + simpl. rewrite IHw1. rewrite IHw2. reflexivity.
-Qed. 
+Qed.
 
 
 (** ** Verification of [Eq1] - NOT COMPLETE*)
