examples/containers/module-edits/Data/IntSet/InternalWord/preamble.v
@@ -1,1 +1,2 @@
-Require BitTerminationProofs.
+Require String BitTerminationProofs.
+Import String.StringSyntax.
